restrict2.v
@@ -1,0 +1,474 @@
+Require Import Utf8_core.
+Require ILLVarInt. (* Don't want import it. *)
+Import ILLVarInt.MILL. (* only this *)
+Import ILLVarInt.M. (* this *)
+Import FormulaMultiSet. (* and this *)
+
+Inductive Istable (pred:∀ e f (h: e ⊢ f), Prop): ∀ e f (h: e ⊢ f) , Prop := 
+| IId: ∀ Γ (f:formula) (heq:Γ == {f}), Istable pred Γ f (Id _ _ heq)
+| IImpl_R: ∀ Γ p q (h:(p :: Γ ⊢ q)), pred _ _ h → Istable pred _ _ (Impl_R Γ p q h)
+| IImpl_L: ∀ Γ Δ Δ' p q r (hin:(p⊸q)∈Γ) (heq:remove (p⊸ q) Γ== Δ ∪ Δ') (h:Δ ⊢ p) (h':q::Δ' ⊢ r), 
+  pred _ _ h → pred _ _ h' → Istable pred _ _ (Impl_L Γ Δ Δ' p q r hin heq h h')
+| ITimes_R: ∀ Γ Δ Δ' p q heq h h', pred _ _ h → pred _ _ h' → Istable pred _ _ (Times_R Γ Δ Δ' p q heq h h')
+| ITimes_L: ∀ Γ p q r hin h, pred _ _ h → Istable pred _ _ (Times_L Γ p q r hin h)
+| IOne_R: ∀ Γ heq, Istable pred _ _ (One_R Γ heq)
+| IOne_L: ∀ Γ p hin h, pred _ _ h → Istable pred _ _ (One_L Γ p hin h)
+| IAnd_R: ∀ Γ p q h h', pred _ _ h → pred _ _ h' → Istable pred _ _ (And_R  Γ p q h h')
+| IAnd_L_2: ∀ Γ p q r hin h, pred _ _ h → Istable pred _ _ (And_L_2 Γ p q r hin h)
+| IAnd_L_1: ∀ Γ p q r hin h, pred _ _ h → Istable pred _ _ (And_L_1 Γ p q r hin h)
+| IOplus_L: ∀ Γ p q r hin h h', pred _ _ h → pred _ _ h' → Istable pred _ _ (Oplus_L  Γ p q r hin h h')
+| IOplus_R_2: ∀ Γ p q h, pred _ _ h  → Istable pred _ _ (Oplus_R_2 Γ p q h)
+| IOplus_R_1: ∀ Γ p q h, pred _ _ h → Istable pred _ _ (Oplus_R_1 Γ p q h)
+(* | IT_ : ∀ Γ,  (pred Γ Top (T_ Γ)) → (Istable pred Γ Top (T_ Γ)) *)
+(* | IZero_: ∀ Γ p truein, (pred Γ p (Zero_ Γ p truein)) → (Istable pred _ _ (Zero_ Γ p truein)) *)
+| IBang_D: ∀ Γ p q hin h, pred _ _ h → (Istable pred _ _ (Bang_D Γ p q hin h))
+| IBang_C: ∀ Γ p q hin h, pred _ _ h → (Istable pred _ _ (Bang_C Γ p q hin h))
+| IBang_W: ∀ Γ p q hin h, pred _ _ h → (Istable pred _ _ (Bang_W Γ p q hin h))
+.
+
+
+
+Inductive A : formula -> Prop :=
+| A1: A 1
+| A2:∀ φ₁ φ₂, Ac φ₁ → Ap φ₂ → A (φ₁ ⊸ φ₂)
+| A3: ∀ φ₁ φ₂, A φ₁ → A φ₂ → A (φ₁ ⊕ φ₂)
+| A4: ∀ φ₁ φ₂, A φ₁ → A φ₂ → A (φ₁ & φ₂)
+| A5: ∀ φ, A φ → A (! φ)
+with Ac: formula -> Prop:=
+| Ac1: Ac 1
+| Ac2: ∀ n, Ac (Proposition n)
+| Ac3: ∀ φ₁ φ₂, Ac φ₁ → Ac φ₂ → Ac (φ₁ ⊗ φ₂)
+with Ap: formula -> Prop:=
+| Ap1:∀ φ, A φ → Ap φ
+| Ap2:∀ φ, R φ → Ap φ
+| Ap3: ∀ φ₁ φ₂, Ap φ₁ → Ap φ₂ → Ap (φ₁ ⊗ φ₂)
+with R: formula -> Prop:=
+  R1: R 1
+| R2: ∀ n, R (Proposition n)
+| R3: ∀ φ, R φ → R (!φ)
+| R4: ∀ φ₁ φ₂, R φ₁ → R φ₂ → R (φ₁ ⊗ φ₂)
+| R5: ∀ φ₁ φ₂, R φ₁ → R φ₂ → R (φ₁ & φ₂)
+.
+
+(*
+Lemma arrto1 : ∀ p q, arr (p ⊸ q) → arr p.
+Proof.
+  intros p q H.
+  inversion H;inversion H0;subst.
+  constructor;assumption.
+Qed.
+
+Lemma arrto2 : ∀ p q, arr (p ⊸ q) → arr q.
+Proof.
+  intros p q H.
+  inversion H;inversion H0;subst.
+  assumption.
+Qed.
+
+
+Lemma arroplus1 : ∀ p q, arr (p ⊕ q) → arr p.
+Proof.
+  intros p q H.
+  inversion H;inversion H0;subst.
+  constructor;assumption.
+Qed.
+
+Lemma arroplus2 : ∀ p q, arr (p ⊕ q) → arr q.
+Proof.
+  intros p q H.
+  inversion H;inversion H0;subst.
+  constructor;assumption.
+Qed.
+
+Lemma arromult1 : ∀ p q, arr (p ⊗ q) → arr p.
+Proof.
+  intros p q H.
+  inversion H;inversion H0;subst.
+  constructor;assumption.
+Qed.
+
+Lemma arromult2 : ∀ p q, arr (p ⊗ q) → arr q.
+Proof.
+  intros p q H.
+  inversion H;inversion H0;subst.
+  constructor;assumption.
+Qed.
+
+
+
+Lemma arroesp1 : ∀ p q, arr (p & q) → arr p.
+Proof.
+  intros p q H.
+  inversion H;inversion H0;subst.
+  constructor;assumption.
+Qed.
+
+Lemma arroesp2 : ∀ p q, arr (p & q) → arr q.
+Proof.
+  intros p q H.
+  inversion H;inversion H0;subst.
+  constructor;assumption.
+Qed.
+*)
+
+Definition Apall Γ f (h:Γ⊢f):Prop := (∀g:formula, g ∈ Γ  → Ap g) /\ Ac f.
+(* Definition Aall2 Γ f (h:Γ⊢f):Prop := (∀g:formula, g ∈ Γ → A g) /\ R f. *)
+  
+(* Axiom A_morph: ∀ Γ p q, Aall Γ (p ⊸ q) → A q. *)
+(* Axiom A_morph: ∀ Γ p q, Aall Γ (p ⊸ q) → A q. *)
+
+Open Scope ILL_scope.
+
+Lemma inEnv:∀ g p Γ,  g ∈ (p :: Γ) → g = p ∨ g ∈ Γ .
+Proof.
+  intros g p Γ H.
+  generalize (mem_destruct _ _ _ H).
+  intros [H1| H1];auto.
+  apply eq_is_eq in H1.
+  auto.
+Qed.  
+
+
+(*Proof.
+  intros g p Γ H.
+
+  Set Printing All.
+  unfold add, add_multiple in H.
+  rewrite (MapsPtes.F.add_in_iff Γ p g 1%nat) in H.
+  unfold Maps'.In , Maps'.Raw.PX.In , Maps'.Raw.PX.MapsTo in H.
+  destruct  H.
+  inversion H.
+
+  unfold add, add_multiple in H0.
+  inversion H0.
+Qed.
+*)
+
+Lemma inAdd1: ∀ f Γ, f ∈ (f :: Γ) .
+Proof.
+  intros f Γ.
+  apply add_is_mem.
+  apply FormulaOrdered.eq_refl.
+Qed.
+
+Lemma inAdd2: ∀ f g Γ, f ∈ Γ → f ∈ (g :: Γ).
+Proof.
+  apply mem_add_is_mem.
+Qed.
+Lemma inUnion1: ∀ g Δ Γ, g ∈ Δ -> g ∈ (Δ ∪ Γ).
+  apply mem_union_l.
+Qed.
+
+Lemma inUnion2: ∀ g Δ Γ, g ∈ Γ -> g ∈ (Δ ∪ Γ).
+  apply mem_union_r.
+Qed.
+
+Lemma inAddUnion1: ∀ g Δ Γ f, g ∈ Δ -> g ∈ (f :: (Δ ∪ Γ)).
+Proof.
+  intros g Δ Γ f H.
+  apply inAdd2.
+  apply inUnion1;assumption.
+Qed.
+Lemma inAddUnion2: ∀ g Δ Γ f, g ∈ Γ -> g ∈ (f :: (Δ ∪ Γ)).
+Proof.
+  intros g Δ Γ f H.
+  apply inAdd2.
+  apply inUnion2;assumption.
+Qed.
+
+Ltac tac :=
+  match goal with
+    | H:?g ∈ ?Δ |- ?g ∈ (_ :: ?Δ ∪ _) => apply inAddUnion1;assumption
+    | H:?g ∈ ?Δ |- ?g ∈ (_ :: _ ∪ ?Δ) => apply inAddUnion2;assumption
+    | H:?g ∈ ?Δ |- ?g ∈ (?Δ ∪ _) => apply inUnion1;assumption
+    | H:?g ∈ ?Δ |- ?g ∈ (_ ∪ ?Δ) => apply inUnion2;assumption
+    | H:(R ?x) |- A ?x => constructor 2;assumption
+    | H:(R (?x ⊸ ?y)) |- _ => inversion H
+    | H:∀ g : formula, g ∈ (_ :: _ ∪ ?Δ) → A g, H':?f ∈ ?Δ |- A ?f => apply H
+    | H:∀ g : formula, g ∈ (_ :: ?Δ ∪ _) → A g, H':?f ∈ ?Δ |- A ?f => apply H
+    | H:∀ g : formula, g ∈ (_ ∪ ?Δ) → A g, H':?f ∈ ?Δ |- A ?f => apply H
+    | H:∀ g : formula, g ∈ (?Δ ∪ _) → A g, H':?f ∈ ?Δ |- A ?f => apply H
+    | H: ∀ g : formula, g ∈ (?f :: _) → A g |- A ?f => apply H
+    | H: ∀ g : formula, g ∈ (?f :: ?Γ) → A g, H': ?f' ∈ ?Γ |- A ?f' => apply H
+    | H : ∀ g : formula, g ∈ ((?p ⊸ ?q) :: ?Γ) → A g |- Ac ?p => 
+      assert (A (p ⊸ q));[ |  assert (∀ g : formula, g ∈ Γ → A g); [ intros |  clear H]]
+    | H : ∀ g : formula, g ∈ ((?p ⊸ ?q) :: ?Γ) → A g |- Ap ?q => 
+      assert (A (p ⊸ q));[ |  assert (∀ g : formula, g ∈ Γ → A g); [ intros |  clear H]]
+    | H : ∀ g : formula, g ∈ ((?p ⊗ ?q) :: ?Γ) → A g |- A ?p => 
+        assert (A (p ⊗ q));[ |  assert (∀ g : formula, g ∈ Γ → A g); [ intros |  clear H]]
+    | H : ∀ g : formula, g ∈ ((?p ⊗ ?q) :: ?Γ) → A g |- A ?q => 
+      assert (A (p ⊗ q));[ |  assert (∀ g : formula, g ∈ Γ → A g); [ intros |  clear H]]
+    | H : ∀ g : formula, g ∈ ((?p ⊕ ?q) :: ?Γ) → A g |- A ?p => 
+        assert (A (p ⊕ q));[ |  assert (∀ g : formula, g ∈ Γ → A g); [ intros |  clear H]]
+    | H : ∀ g : formula, g ∈ ((?p ⊕ ?q) :: ?Γ) → A g |- A ?q => 
+      assert (A (p ⊕ q));[ |  assert (∀ g : formula, g ∈ Γ → A g); [ intros |  clear H]]
+    | H : ∀ g : formula, g ∈ ((?p & ?q) :: ?Γ) → A g |- A ?p => 
+        assert (A (p & q));[ |  assert (∀ g : formula, g ∈ Γ → A g); [ intros |  clear H]]
+    | H : ∀ g : formula, g ∈ ((?p & ?q) :: ?Γ) → A g |- A ?q => 
+      assert (A (p & q));[ |  assert (∀ g : formula, g ∈ Γ → A g); [ intros |  clear H]]
+    | H : ∀ g : formula, g ∈ ((!?p) :: ?Γ) → A g |- A ?p => 
+      assert (A (!p));[ |  assert (∀ g : formula, g ∈ Γ → A g); [ intros |  clear H]]
+    | |- ?g ∈ (?g :: ?Γ) => apply inAdd1 (* will try stupid cases *)
+    | H:?g ∈ ?Γ |- ?g ∈ (?f :: ?Γ) => apply inAdd2;assumption
+    | H:?g ∈ (?p :: ?Γ) |- A ?g => destruct (inEnv g p Γ);auto;subst;clear H
+    | |- A (?p ⊕ ?q) => constructor
+    | |- A (?p ⊸ ?q) => constructor
+    | |- A (?p ⊗ ?q) => constructor
+    | |- A (?p & ?q) => constructor
+    | |- R ?p => constructor
+  end.
+
+(* Axiom memIn: ∀ x (y:env), Maps'.mem x y = true → Maps'.In x y. *)
+
+Lemma notA0 : ~ (A 0).
+Proof.
+  intro H.
+  inversion H.
+Qed.
+
+
+Scheme A_ind' := Induction for A Sort Prop
+with Ac_ind' := Induction for Ac Sort Prop
+with Ap_ind' := Induction for Ap Sort Prop
+with R_ind' := Induction for R Sort Prop.
+
+
+Lemma eq_A_morph: ∀ f, A f → ∀ f', ILLVarInt.MILL.eq f' f →  A f'.
+Proof.
+  intros f H.
+  induction H using A_ind' with (P0:= λ f H, ∀f', Ac f → ILLVarInt.MILL.eq f f' →  Ac f') (P1:= λ f H, ∀f', Ap f → ILLVarInt.MILL.eq f f' →  Ap f') (P2:= λ f H, ∀f', R f → ILLVarInt.MILL.eq f f' →  R f');intros.
+
+  destruct f' ;intros;simpl in *;try (subst;contradiction);  simpl in *; intuition ; constructor;auto. 
+  destruct f' ;intros;simpl in *;try (subst;contradiction);  simpl in *; intuition ; constructor;auto. 
+  destruct f' ;intros;simpl in *;try (subst;contradiction);  simpl in *; intuition ; constructor;auto. 
+  destruct f' ;intros;simpl in *;try (subst;contradiction);  simpl in *; intuition ; constructor;auto. 
+  destruct f' ;intros;simpl in *;try (subst;contradiction);  simpl in *; intuition ; constructor;auto. 
+  destruct f' ;intros;simpl in *;try (subst;contradiction);  simpl in *; intuition ; constructor;auto. 
+  destruct f' ;intros;simpl in *;try (subst;contradiction);  simpl in *; intuition ; constructor;auto. 
+  destruct f' ;intros;simpl in *;try (subst;contradiction);  simpl in *; intuition ; constructor;auto. 
+  destruct f' ;intros;simpl in *;try (subst;contradiction);  simpl in *; intuition ; constructor;auto. 
+  constructor 2. auto.
+  destruct f' ;intros;simpl in *;try (subst;contradiction);  simpl in *; intuition ; constructor 3;auto. 
+  destruct f' ;intros;simpl in *;try (subst;contradiction);  simpl in *; intuition ; constructor;auto. 
+  destruct f' ;intros;simpl in *;try (subst;contradiction);  simpl in *; intuition ; constructor;auto. 
+  destruct f' ;intros;simpl in *;try (subst;contradiction);  simpl in *; intuition ; constructor;auto. 
+  destruct f' ;intros;simpl in *;try (subst;contradiction);  simpl in *; intuition ; constructor;auto. 
+  destruct f' ;intros;simpl in *;try (subst;contradiction);  simpl in *; intuition ; constructor;auto. 
+Qed.  
+
+
+Lemma eq_Ap_morph: ∀ f, Ap f → ∀ f', ILLVarInt.MILL.eq f' f →  Ap f'.
+Proof.
+  intros f H.
+  induction H using Ap_ind' with (P:= λ f H, ∀f', A f → ILLVarInt.MILL.eq f f' →  A f') (P0:= λ f H, ∀f', Ac f → ILLVarInt.MILL.eq f f' →  Ac f') (P2:= λ f H, ∀f', R f → ILLVarInt.MILL.eq f f' →  R f');intros.
+
+  destruct f' ;intros;simpl in *;try (subst;contradiction);  simpl in *; intuition ; constructor;auto. 
+  destruct f' ;intros;simpl in *;try (subst;contradiction);  simpl in *; intuition ; constructor;auto. 
+  destruct f' ;intros;simpl in *;try (subst;contradiction);  simpl in *; intuition ; constructor;auto. 
+  destruct f' ;intros;simpl in *;try (subst;contradiction);  simpl in *; intuition ; constructor;auto. 
+  destruct f' ;intros;simpl in *;try (subst;contradiction);  simpl in *; intuition ; constructor;auto. 
+  destruct f' ;intros;simpl in *;try (subst;contradiction);  simpl in *; intuition ; constructor;auto. 
+  destruct f' ;intros;simpl in *;try (subst;contradiction);  simpl in *; intuition ; constructor;auto. 
+  destruct f' ;intros;simpl in *;try (subst;contradiction);  simpl in *; intuition ; constructor;auto. 
+  destruct f' ;intros;simpl in *;try (subst;contradiction);  simpl in *; intuition ; constructor;auto. 
+  constructor 2. auto.
+  destruct f' ;intros;simpl in *;try (subst;contradiction);  simpl in *; intuition . constructor 3;auto. 
+  destruct f' ;intros;simpl in *;try (subst;contradiction);  simpl in *; intuition ; constructor;auto. 
+  destruct f' ;intros;simpl in *;try (subst;contradiction);  simpl in *; intuition ; constructor;auto. 
+  destruct f' ;intros;simpl in *;try (subst;contradiction);  simpl in *; intuition ; constructor;auto. 
+  destruct f' ;intros;simpl in *;try (subst;contradiction);  simpl in *; intuition ; constructor;auto. 
+  destruct f' ;intros;simpl in *;try (subst;contradiction);  simpl in *; intuition ; constructor;auto. 
+Qed.  
+
+
+Lemma eq_Ac_morph: ∀ f, Ac f → ∀ f', ILLVarInt.MILL.eq f' f →  Ac f'.
+Proof.
+  intros f H.
+  induction H using Ac_ind' with (P:= λ f H, ∀f', A f → ILLVarInt.MILL.eq f f' →  A f') (P1:= λ f H, ∀f', Ap f → ILLVarInt.MILL.eq f f' →  Ap f') (P2:= λ f H, ∀f', R f → ILLVarInt.MILL.eq f f' →  R f');intros.
+
+  destruct f' ;intros;simpl in *;try (subst;contradiction);  simpl in *; intuition ; constructor;auto. 
+  destruct f' ;intros;simpl in *;try (subst;contradiction);  simpl in *; intuition ; constructor;auto. 
+  destruct f' ;intros;simpl in *;try (subst;contradiction);  simpl in *; intuition ; constructor;auto. 
+  destruct f' ;intros;simpl in *;try (subst;contradiction);  simpl in *; intuition ; constructor;auto. 
+  destruct f' ;intros;simpl in *;try (subst;contradiction);  simpl in *; intuition ; constructor;auto. 
+  destruct f' ;intros;simpl in *;try (subst;contradiction);  simpl in *; intuition ; constructor;auto. 
+  destruct f' ;intros;simpl in *;try (subst;contradiction);  simpl in *; intuition ; constructor;auto. 
+  destruct f' ;intros;simpl in *;try (subst;contradiction);  simpl in *; intuition ; constructor;auto. 
+  destruct f' ;intros;simpl in *;try (subst;contradiction);  simpl in *; intuition ; constructor;auto. 
+  constructor 2. auto.
+  destruct f' ;intros;simpl in *;try (subst;contradiction);  simpl in *; intuition . constructor 3;auto. 
+  destruct f' ;intros;simpl in *;try (subst;contradiction);  simpl in *; intuition ; constructor;auto. 
+  destruct f' ;intros;simpl in *;try (subst;contradiction);  simpl in *; intuition ; constructor;auto. 
+  destruct f' ;intros;simpl in *;try (subst;contradiction);  simpl in *; intuition ; constructor;auto. 
+  destruct f' ;intros;simpl in *;try (subst;contradiction);  simpl in *; intuition ; constructor;auto. 
+  destruct f' ;intros;simpl in *;try (subst;contradiction);  simpl in *; intuition ; constructor;auto. 
+Qed.  
+
+Lemma eq_R_morph: ∀ f, R f → ∀ f', ILLVarInt.MILL.eq f' f →  R f'.
+Proof.
+  intros f H.
+  induction H using R_ind' with (P:= λ f H, ∀f', A f → ILLVarInt.MILL.eq f f' →  A f') (P1:= λ f H, ∀f', Ap f → ILLVarInt.MILL.eq f f' →  Ap f') (P0:= λ f H, ∀f', Ac f → ILLVarInt.MILL.eq f f' →  Ac f');intros.
+
+  destruct f' ;intros;simpl in *;try (subst;contradiction);  simpl in *; intuition ; constructor;auto. 
+  destruct f' ;intros;simpl in *;try (subst;contradiction);  simpl in *; intuition ; constructor;auto. 
+  destruct f' ;intros;simpl in *;try (subst;contradiction);  simpl in *; intuition ; constructor;auto. 
+  destruct f' ;intros;simpl in *;try (subst;contradiction);  simpl in *; intuition ; constructor;auto. 
+  destruct f' ;intros;simpl in *;try (subst;contradiction);  simpl in *; intuition ; constructor;auto. 
+  destruct f' ;intros;simpl in *;try (subst;contradiction);  simpl in *; intuition ; constructor;auto. 
+  destruct f' ;intros;simpl in *;try (subst;contradiction);  simpl in *; intuition ; constructor;auto. 
+  destruct f' ;intros;simpl in *;try (subst;contradiction);  simpl in *; intuition ; constructor;auto. 
+  destruct f' ;intros;simpl in *;try (subst;contradiction);  simpl in *; intuition ; constructor;auto. 
+  constructor 2. auto.
+  destruct f' ;intros;simpl in *;try (subst;contradiction);  simpl in *; intuition . constructor 3;auto. 
+  destruct f' ;intros;simpl in *;try (subst;contradiction);  simpl in *; intuition ; constructor;auto. 
+  destruct f' ;intros;simpl in *;try (subst;contradiction);  simpl in *; intuition ; constructor;auto. 
+  destruct f' ;intros;simpl in *;try (subst;contradiction);  simpl in *; intuition ; constructor;auto. 
+  destruct f' ;intros;simpl in *;try (subst;contradiction);  simpl in *; intuition ; constructor;auto. 
+  destruct f' ;intros;simpl in *;try (subst;contradiction);  simpl in *; intuition ; constructor;auto. 
+Qed.  
+
+
+
+Lemma essai : ∀ Γ φ (h:Γ ⊢ φ), Apall Γ φ h → Istable Apall _ _ h.
+Proof.
+  intros Γ φ h.
+  destruct h;
+    intros; try constructor;try (unfold Apall in *;decompose [and] H;clear H); try split;intros;auto;
+      try solve [ progress repeat progress tac;auto ];
+        try match goal with
+          | H:Ac _ |- _ => solve [inversion H]
+          | H:A _ |- _ => solve [inversion H]
+          | H:Ap _ |- _ => solve [inversion H]
+          | H:R _ |- _ => solve [inversion H]
+        end.
+  apply H0.
+  admit.
+  assert (Ap (p ⊸ q)) by auto.
+  repeat match goal with
+    | H:Ap (p ⊸ q) |- _ => inversion H;clear H
+    | H:A (p ⊸ q) |- _ => inversion H;clear H
+    | H:R (p ⊸ q) |- _ => inversion H;clear H
+         end;try assumption.
+  
+  destruct (mem_destruct _ _ _ H) as [H3| H3];clear H.
+  apply eq_is_eq in H3;subst.
+  assert (Ap (p ⊸ q)) by auto.
+  repeat match goal with
+    | H:Ap (p ⊸ q) |- _ => inversion H;clear H
+    | H:A (p ⊸ q) |- _ => inversion H;clear H
+    | H:R (p ⊸ q) |- _ => inversion H;clear H
+         end;try assumption.
+  apply H0.
+  admit.
+
+***
+
+  setoid_rewrite  H2 in H1.
+  apply eq_is_eq in H2;subst.
+  assert (h':A (p ⊗ q)).
+  auto.
+  inversion h';clear h';subst.
+  inversion H;constructor assumption.
+  destruct (mem_destruct _ _ _ H2) as [H3| H3];clear H2.
+  apply eq_is_eq in H3;subst.
+  assert (h':A (p ⊗ q)) by  auto.
+  inversion h';clear h';subst.
+  inversion H;constructor assumption.
+  apply mem_remove_2 in H3;auto.
+  
+  
+  apply H0. 
+  apply mem_union_l with (ms':=Δ') in H.
+  rewrite <- e0 in H.
+  eapply mem_remove_2;eexact H.
+  
+  assert (h:A (p ⊸ q)).
+  apply H0;assumption.
+  inversion h;clear h;subst.
+  constructor assumption.
+  inversion H.
+
+  destruct (mem_destruct _ _ _ H);clear H.
+  apply eq_is_eq in H2;subst.
+  assert (h:A (p ⊸ q)).
+  apply H0;assumption.
+  inversion h;clear h;subst.
+  assumption.
+  inversion H.
+
+  apply H0. 
+  apply mem_union_r with (ms:=Δ) in H2.
+  rewrite <- e0 in H2.
+  eapply mem_remove_2;eexact H2.
+
+  apply H0. 
+  apply mem_union_l with (ms':=Δ') in H.
+  rewrite <- e in H;assumption.
+
+  apply H0. 
+  apply mem_union_r with (ms:=Δ) in H.
+  rewrite <- e in H;assumption.
+
+  destruct (mem_destruct _ _ _ H) as [H2| H2];clear H.
+  apply eq_is_eq in H2;subst.
+  assert (h':A (p ⊗ q)).
+  auto.
+  inversion h';clear h';subst.
+  inversion H;constructor assumption.
+  destruct (mem_destruct _ _ _ H2) as [H3| H3];clear H2.
+  apply eq_is_eq in H3;subst.
+  assert (h':A (p ⊗ q)) by  auto.
+  inversion h';clear h';subst.
+  inversion H;constructor assumption.
+  apply mem_remove_2 in H3;auto.
+
+  apply mem_remove_2 in H;auto.
+
+  destruct (mem_destruct _ _ _ H) as [H3| H3];clear H.
+  apply eq_is_eq in H3;subst.
+  assert (h':A (p & q)) by  auto.
+  inversion h';clear h';subst.
+  inversion H;constructor assumption.
+  apply mem_remove_2 in H3;auto.
+
+
+  destruct (mem_destruct _ _ _ H) as [H3| H3];clear H.
+  apply eq_is_eq in H3;subst.
+  assert (h':A (p & q)) by  auto.
+  inversion h';clear h';subst.
+  inversion H;constructor assumption.
+  apply mem_remove_2 in H3;auto.
+
+  destruct (mem_destruct _ _ _ H) as [H3| H3];clear H.
+  apply eq_is_eq in H3;subst.
+  assert (h':A (p ⊕ q)) by  auto.
+  inversion h';clear h';subst.
+  inversion H;constructor assumption.
+  apply mem_remove_2 in H3;auto.
+
+  destruct (mem_destruct _ _ _ H) as [H3| H3];clear H.
+  apply eq_is_eq in H3;subst.
+  assert (h':A (p ⊕ q)) by  auto.
+  inversion h';clear h';subst.
+  inversion H;constructor assumption.
+  apply mem_remove_2 in H3;auto.
+
+  inversion H1.
+  inversion H.
+
+  assert (A 0) by auto.
+  inversion H.
+  inversion H2.
+  
+  destruct (mem_destruct _ _ _ H) as [H3| H3];clear H.
+  apply eq_is_eq in H3;subst.
+  assert (h':A (!p)) by  auto.
+  inversion h';clear h';subst.
+  inversion H;constructor assumption.
+  apply mem_remove_2 in H3;auto.
+
+  apply mem_remove_2 in H;auto.
+
+Qed.  
+
+
